mppa_k1c/TargetPrinter.ml
@@ -294,6 +294,8 @@ module Target (*: TARGET*) =
          fprintf oc "	sxwd	%a = %a\n" ireg rd ireg rs
       | Pzxwd(rd, rs) ->
          fprintf oc "	zxwd	%a = %a\n" ireg rd ireg rs
+      | Pfloatwrnsz(rd, rs) ->
+         fprintf oc "	floatw.rn.s	%a = %a, 0\n" ireg rd ireg rs
 
       (* Arith RI32 instructions *)
       | Pmake (rd, imm) ->
